SHA256_elim QED

demos/sha256/SHA256_elim.v
@@ -890,6 +890,13 @@ rewrite N.shiftl_mul_pow2, N.shiftr_div_pow2.
 reflexivity.
 Qed.
 
+Lemma generate_and_pad_length : forall msg,
+    (length (generate_and_pad msg) mod 16 = 0)%nat.
+intros.
+rewrite generate_and_pad_eq.
+apply SHA256_N.generate_and_pad_length.
+Qed.
+
 
 Definition nthi_test n :=
     (nat_rect _ (fun dummy => 10)
@@ -1264,26 +1271,6 @@ induction t; intros0 HM; unfold Round; cbn [nat_rect].
 Qed.
 
 
-Definition hash_block_inner (block : list N)
-        a0 b0 c0 d0 e0 f0 g0 h0 :=
-    prod_rect (fun _ => registers) (fun abcdefg1 h1 =>
-    prod_rect (fun _ => registers) (fun abcdef1 g1 =>
-    prod_rect (fun _ => registers) (fun abcde1 f1 =>
-    prod_rect (fun _ => registers) (fun abcd1 e1 =>
-    prod_rect (fun _ => registers) (fun abc1 d1 =>
-    prod_rect (fun _ => registers) (fun ab1 c1 =>
-    prod_rect (fun _ => registers) (fun a1 b1 =>
-        (t_add a0 a1,
-         t_add b0 b1,
-         t_add c0 c1,
-         t_add d0 d1,
-         t_add e0 e1,
-         t_add f0 f1,
-         t_add g0 g1,
-         t_add h0 h1)
-    ) ab1) abc1) abcd1) abcde1) abcdef1) abcdefg1)
-        (Round (a0, b0, c0, d0, e0, f0, g0, h0) (nthi block) 63).
-
 Definition hash_block (r : registers) (block : list N) : registers :=
     prod_rect (fun _ => registers) (fun abcdefg0 h0 =>
     prod_rect (fun _ => registers) (fun abcdef0 g0 =>
@@ -1310,51 +1297,6 @@ Definition hash_block (r : registers) (block : list N) : registers :=
     ) ab1) abc1) abcd1) abcde1) abcdef1) abcdefg1) (Round r (nthi block) 63)
     ) ab0) abc0) abcd0) abcde0) abcdef0) abcdefg0) r.
 
-Lemma add_8_eq : forall
-        a0 b0 c0 d0 e0 f0 g0 h0
-        a1 b1 c1 d1 e1 f1 g1 h1,
-    (t_add a0 a1,
-     t_add b0 b1,
-     t_add c0 c1,
-     t_add d0 d1,
-     t_add e0 e1,
-     t_add f0 f1,
-     t_add g0 g1,
-     t_add h0 h1) =
-    (SHA256_N.t_add a0 a1,
-     SHA256_N.t_add b0 b1,
-     SHA256_N.t_add c0 c1,
-     SHA256_N.t_add d0 d1,
-     SHA256_N.t_add e0 e1,
-     SHA256_N.t_add f0 f1,
-     SHA256_N.t_add g0 g1,
-     SHA256_N.t_add h0 h1).
-intros.
-rewrite 8 t_add_eq.
-reflexivity.
-Qed.
-
-Lemma hash_block_inner_eq : forall block 
-        a0 b0 c0 d0 e0 f0 g0 h0,
-    hash_block_inner block a0 b0 c0 d0 e0 f0 g0 h0 =
-    let '(a1, b1, c1, d1, e1, f1, g1, h1) :=
-        SHA256_N.Round (a0, b0, c0, d0, e0, f0, g0, h0) (SHA256_N.nthi block) 63 in
-    (SHA256_N.t_add a0 a1,
-     SHA256_N.t_add b0 b1,
-     SHA256_N.t_add c0 c1,
-     SHA256_N.t_add d0 d1,
-     SHA256_N.t_add e0 e1,
-     SHA256_N.t_add f0 f1,
-     SHA256_N.t_add g0 g1,
-     SHA256_N.t_add h0 h1).
-intros.
-unfold hash_block_inner.
-erewrite Round_eq by eapply nthi_eq.
-destruct (SHA256_N.Round _ _ _) as [[[[[[[a1 b1] c1] d1] e1] f1] g1] h1].
-cbn [prod_rect].
-apply add_8_eq.
-Qed.
-
 Opaque Round t_add nthi.
 Opaque SHA256_N.Round SHA256_N.t_add SHA256_N.nthi.
 Lemma hash_block_eq : forall r block,
@@ -1368,3 +1310,129 @@ rewrite 8 t_add_eq. reflexivity.
 Qed.
 Transparent Round t_add nthi.
 Transparent SHA256_N.Round SHA256_N.t_add SHA256_N.nthi.
+
+
+Definition pairs_to_list_16 x : list N :=
+    prod_rect (fun _ => list N) (fun x0 x1 =>
+
+    prod_rect (fun _ => list N) (fun x00 x01 =>
+    prod_rect (fun _ => list N) (fun x10 x11 =>
+
+    prod_rect (fun _ => list N) (fun x000 x001 =>
+    prod_rect (fun _ => list N) (fun x010 x011 =>
+    prod_rect (fun _ => list N) (fun x100 x101 =>
+    prod_rect (fun _ => list N) (fun x110 x111 =>
+
+    prod_rect (fun _ => list N) (fun x0000 x0001 =>
+    prod_rect (fun _ => list N) (fun x0010 x0011 =>
+    prod_rect (fun _ => list N) (fun x0100 x0101 =>
+    prod_rect (fun _ => list N) (fun x0110 x0111 =>
+    prod_rect (fun _ => list N) (fun x1000 x1001 =>
+    prod_rect (fun _ => list N) (fun x1010 x1011 =>
+    prod_rect (fun _ => list N) (fun x1100 x1101 =>
+    prod_rect (fun _ => list N) (fun x1110 x1111 =>
+
+    [x0000; x0001; x0010; x0011;
+     x0100; x0101; x0110; x0111;
+     x1000; x1001; x1010; x1011;
+     x1100; x1101; x1110; x1111]
+
+    ) x111) x110) x101) x100) x011) x010) x001) x000
+    ) x11) x10) x01) x00
+    ) x1) x0
+    ) x.
+
+(* used for verification only *)
+Definition hash_blocks' (r : registers) msg_blocks : registers :=
+    list_rect _
+        (fun r => r)
+        (fun block msg IHmsg => fun r =>
+            IHmsg (hash_block r (pairs_to_list_16 block)))
+        msg_blocks r.
+
+Definition hash_blocks (r : registers) (msg : list N) : registers :=
+    list_rect _
+        (fun r => r)
+        (fun block msg IHmsg => fun r =>
+            IHmsg (hash_block r (pairs_to_list_16 block)))
+        (pair_up (pair_up (pair_up (pair_up msg)))) r.
+
+Lemma hash_blocks'_unfold_cons : forall r block blocks,
+    hash_blocks' r (block :: blocks) = hash_blocks' (hash_block r (pairs_to_list_16 block)) blocks.
+intros. reflexivity.
+Qed.
+
+Lemma pair_up_unfold_cons : forall {A} (x1 x2 : A) xs,
+    pair_up (x1 :: x2 :: xs) = (x1, x2) :: pair_up xs.
+intros. reflexivity.
+Qed.
+
+Lemma hash_blocks_eq : forall r msg,
+    (length msg mod 16 = 0)%nat ->
+    hash_blocks r msg = SHA256_N.hash_blocks r msg.
+intros0 Hlen.
+unfold hash_blocks. fold (hash_blocks' r (pair_up (pair_up (pair_up (pair_up msg))))).
+remember (pair_up _) as msg_p.
+revert msg_p msg r Hlen Heqmsg_p. induction msg_p; intros.
+
+- do 16 try destruct msg as [| ?m0 msg ].
+  (* empty msg *)
+    { reflexivity. }
+
+  (* uneven-length messages *)
+    all: try solve [exfalso; simpl in Hlen; discriminate Hlen].
+
+  (* impossible - nil = cons *)
+    { exfalso. repeat rewrite pair_up_unfold_cons in Heqmsg_p. discriminate. }
+
+- rewrite hash_blocks'_unfold_cons.
+
+  do 16 try destruct msg as [| ?m0 msg ].
+  (* empty msg *)
+    { discriminate Heqmsg_p. }
+  (* uneven-length messages *)
+    all: try solve [exfalso; simpl in Hlen; discriminate Hlen].
+
+  (* remaining case: nonempty message of appropriate length *)
+  repeat rewrite pair_up_unfold_cons in Heqmsg_p.
+  change (length _) with (16 + length msg)%nat in Hlen.
+  invc Heqmsg_p. simpl.
+  rewrite hash_block_eq.
+  eapply IHmsg_p; eauto.
+
+  + rewrite Nat.add_mod in Hlen by discriminate.
+    change (16 mod 16)%nat with (0 mod 16)%nat in Hlen.
+    rewrite <- Nat.add_mod in Hlen by discriminate.
+    exact Hlen.
+Qed.
+
+
+Definition SHA_256 (str : list N) : list N :=
+    prod_rect (fun _ => list N) (fun abcdefg h =>
+    prod_rect (fun _ => list N) (fun abcdef g =>
+    prod_rect (fun _ => list N) (fun abcde f =>
+    prod_rect (fun _ => list N) (fun abcd e =>
+    prod_rect (fun _ => list N) (fun abc d =>
+    prod_rect (fun _ => list N) (fun ab c =>
+    prod_rect (fun _ => list N) (fun a b =>
+    wordlist_to_bytelist [a; b; c; d; e; f; g; h]
+    ) ab) abc) abcd) abcde) abcdef) abcdefg)
+    (hash_blocks 
+        (* init_registers *)
+        (1779033703, 3144134277, 1013904242, 2773480762,
+         1359893119, 2600822924,  528734635, 1541459225)%N
+     (generate_and_pad str)).
+
+Lemma SHA_256_eq : forall str,
+    SHA_256 str = SHA256_N.SHA_256 str.
+intros.
+unfold SHA_256.
+rewrite generate_and_pad_eq.
+rewrite hash_blocks_eq.
+fold SHA256_N.init_registers.
+
+unfold SHA256_N.SHA_256.
+destruct (SHA256_N.hash_blocks _ _) as [[[[[[[a b] c] d] e] f] g] h].
+cbn [prod_rect]. apply wordlist_to_bytelist_eq.
+apply SHA256_N.generate_and_pad_length.
+Qed.
